Using reduce to fit with the expected representation of maps as association lists.

theories/newth/NewFMap.ec
@@ -7,12 +7,6 @@ require import Fun Pred Option Pair Int NewList NewFSet.
 
 pragma +implicits.
 
-(*
-op reduce (xs : ('a * 'b) list) : ('a * 'b) list =
-  foldl (fun aout (kv : 'a * 'b) =>
-    if mem [] kv.`1 then aout else kv :: aout)
-  [] xs. *)
-
 (** Even more general (to NewList?) **)
 lemma uniq_map_uniq (xs : 'a list) (f : 'a -> 'c):
   uniq (map f xs) => uniq xs.
@@ -28,43 +22,74 @@ proof. by move=> /(perm_eq_map f) /perm_eq_uniq ->. qed.
 
 (* TODO: this may be of more general interest and may benefit from a
          move to NewList, or a separate PairList theory. *)
-op undup_fst (xs : ('a * 'b) list) =
-  with xs = "[]"      => []
-  with xs = (::) x xs => if mem (map fst xs) x.`1
-                         then undup_fst xs
-                         else x::undup_fst xs.
-
 lemma mem_fst_ex_snd (xs : ('a * 'b) list) (x : 'a):
   mem (map fst xs) x <=> (exists y, mem xs (x,y)).
 proof.
   rewrite -has_pred1 has_map hasP /preim/fst/pred1; split.
-    by move=> [[a b]] [x0_in_xs ->>]; exists b.
+    by move=> [[a b]] /= [x0_in_xs ->>]; exists b.
   by move=> [y] xs_in_xs; exists (x,y).
 qed.
 
 lemma mem_snd_ex_fst (xs : ('a * 'b) list) (y : 'b):
   mem (map snd xs) y <=> (exists x, mem xs (x,y)).
 proof.
-  rewrite -has_pred1 has_map hasP /preim/fst/pred1; split.
-    by move=> [[a b]] [x0_in_xs ->>]; exists a.
+  rewrite -has_pred1 has_map hasP /preim/snd/pred1; split.
+    by move=> [[a b]] /= [x0_in_xs ->>]; exists a.
   by move=> [x] xs_in_xs; exists (x,y).
 qed.
 
-lemma mem_fst_undup_fst (xs : ('a * 'b) list):
-  mem (map fst (undup_fst xs)) <= mem (map fst xs).
+op reduce_witness (xs : ('a * 'b) list): 'a list * ('a * 'b) list =
+  foldl (fun (aout : 'a list * ('a * 'b) list) (kv : 'a * 'b) =>
+           if mem aout.`1 kv.`1 then aout else (rcons aout.`1 kv.`1,rcons aout.`2 kv))
+        ([],[]) xs.
+
+lemma mem_reduce_witness (xs : ('a * 'b) list):
+   mem (reduce_witness xs).`1 = mem (map fst xs).
 proof.
-  elim xs=> //= x xs IH.
-  case (mem (map fst xs) x.`1).
-    by move=> x1_in_fstxs a /IH; rewrite in_cons=> ->.
-    by move=> x1_notin_fstxs a; rewrite !in_cons=> [-> | /IH ->].
+  rewrite /reduce_witness -{1}@(revK xs) foldl_rev.
+  rewrite -{2}@(cats0 xs).
+  cut: [<:'a>] = map fst [<:'a*'b>] by done.
+  move: [<:'a>] [<:'a*'b>]; elim xs=> //=.
+    by rewrite /rev //= => acc acc'.
+  move=> x xs IH a a' H.
+  rewrite /rev /= catrevE foldr_cat /= /=.
+  case (mem a x.`1).
+    rewrite (IH a a' _) // => x1_in_a.
+    subst a; apply fun_ext=> x'.
+    rewrite in_cons map_cat mem_cat; case (x' = fst x)=> //=.
+    by move=> ->; rewrite x1_in_a.
+  cut ->:= IH (rcons a x.`1) (rcons a' x) _.
+    by rewrite map_rcons -H.
+  move=> x1_notin_a; apply fun_ext=> x'.
+  rewrite !(in_cons,map_cat,mem_cat,map_rcons,mem_rcons).
+  smt. (* Parce que je le vaux bien. *)
 qed.
 
-lemma uniq_undup_fst (xs : ('a * 'b) list): uniq (map fst (undup_fst xs)).
+lemma reduce_witness_projs (xs : ('a * 'b) list):
+  map fst (reduce_witness xs).`2 = (reduce_witness xs).`1.
 proof.
-  elim xs=> //= x xs IH.
-  case (mem (map fst xs) x.`1)=> //=.
-  rewrite IH /= => x1_notin_fstundup.
-  by rewrite -not_def=> /mem_fst_undup_fst.
+  rewrite /reduce_witness.
+  cut: map fst (([<:'a>],[<:'a*'b>]).`2) = ([<:'a>],[<:'a*'b>]).`1 by done.
+  elim xs [<:'a>] [<:'a*'b>]=> //= x xs IH a a' a_eq_fa'.
+  case (mem a x.`1)=> //=.
+    by rewrite (IH a a' a_eq_fa').
+  cut -> //:= IH (rcons a x.`1) (rcons a' x) _.
+  by rewrite map_rcons a_eq_fa'.
+qed.  
+
+op reduce (xs : ('a * 'b) list): ('a * 'b) list =
+  (reduce_witness xs).`2.
+
+lemma mem_fst_reduce (xs : ('a * 'b) list):
+  mem (map fst (reduce xs)) = mem (map fst xs).
+proof.
+  rewrite /reduce -@(mem_reduce_witness xs).
+  by cut ->:= reduce_witness_projs xs. (* Why not rewrite? BECAUSE IT DOES NOT WORK! :) *)
+qed.
+
+lemma uniq_fst_reduce (xs : ('a * 'b) list): uniq (map fst (reduce xs)).
+proof.
+  admit. (** TODO: Adapt this proof to using reduce **)
 qed.
 
 lemma uniq_perm_eq_map (s1 s2 : ('a * 'b) list) (f: 'a * 'b -> 'c):
@@ -87,14 +112,14 @@ op elems  : ('a,'b) fmap -> ('a * 'b) list.
 op oflist : ('a * 'b) list -> ('a,'b) fmap.
 
 axiom elemsK  (m : ('a,'b) fmap): Self.oflist (elems  m) = m.
-axiom oflistK (s : ('a * 'b) list): perm_eq (undup_fst s) (elems (Self.oflist s)).
+axiom oflistK (s : ('a * 'b) list): perm_eq (reduce s) (elems (Self.oflist s)).
 
 lemma uniq_keys (m : ('a,'b) fmap): uniq (map fst (elems m)).
 proof.
   rewrite -elemsK; move: (elems m) => {m} m.
-  apply @(perm_eq_uniq (map fst (undup_fst m)) _).
+  apply @(perm_eq_uniq (map fst (reduce m)) _).
     by apply perm_eq_map; apply oflistK.
-  by apply uniq_undup_fst.
+  by apply uniq_fst_reduce.
 qed.
 
 axiom fmap_eq (s1 s2 : ('a,'b) fmap):
